state/README.md
@@ -1,6 +1,4 @@
 # TODO: prove assumptions
 - [ ] Properties of footprint in `TargetLangIFC`: `footprint_modifies_none` and `footprint_cons`
 - [ ] Prove assumptions necessary for `progr_high_ll_unchanged_separation` and `ll_constant_trans`.
-- [ ] `write'`, `_alloc`, `declassify_low'`, `alloc'` in `TargetLangIFC` --- one could use the same strategy to prove all of them
-- [ ] `lemma_modifies_only_label_trans` in `IFC.Heap.ST`
-- [ ] `inversion` in `TargetLangIFC` --- we cannot prove this without some workarounds
+- [ ] `inversion` in `Translation` --- we cannot prove this without some workarounds
